to_N_path

cleanup/Downward.v
@@ -1,5 +1,3 @@
-
-
 Require Import Coq.Strings.String Coq.Bool.Bool Coq.Lists.List.
 Import ListNotations.
 From Coq.Arith Require Import Arith EqNat.
@@ -9,3 +7,19 @@ Require Import Coq.Program.Equality.
 Require Import Arith.
 Require Import Coq.Program.Tactics.
 From Taxiway Require Import To_naive.
+From Taxiway Require Import Find_path.
+From Taxiway Require Import Correctness.
+
+From Hammer Require Import Hammer.
+
+(* This file have five theorems indicating the theorem of complete graph preserve downward*)
+
+Definition naive_path_starts_with_vertex (path : list Edge_type) (start_v : Vertex) : Prop := 
+    exists taxiway_name, exists l, path = ((start_v, input), taxiway_name) :: l.
+
+
+Theorem naive_start_correct:
+    forall start_v end_v ATC D (path : list Arc_type) (paths : list (list Arc_type)),
+    Some paths = (find_path (start_v : Vertex) (end_v : Vertex) (ATC : list string) (D : C_Graph_type)) ->
+    In path (to_N paths) ->
+    naive_path_starts_with_vertex path start_v.
