cleanup/To_naive.v
@@ -82,8 +82,15 @@ Defined.
 
 
 Definition to_N (le : list Arc_type) : list Edge_type := 
-    nodup dec_Edge (map (fun ce => (ce.1.2, ce.2)) le).
+    (map (fun ce => (ce.1.2, ce.2)) le).
 
-(*Eval compute in to_N [(((Ch, BC), (Ch, AA3)), B); (((Ch, BC), (Ch, AA3)), B)].
+
+(* Since we can't apply nodup to path, 
+    because we might encounter cases going through on edge multiple times*)
+Definition to_N_path (le : list Arc_type) : list Edge_type :=
+    map (fun ce => (ce.1.2, ce.2)) le.
+
+
+(* Eval compute in to_N [(((Ch, BC), (Ch, AA3)), B); (((Ch, BC), (Ch, AA3)), B)].
 Example xm : to_N [(((Ch, BC), (Ch, AA3)), B); (((Ch, BC), (Ch, AA3)), B)] = [((Ch, AA3), B)].
 Proof. compute. reflexivity. Qed. *)
